\documentclass{ximera}

\begin{document}
	\author{Stitz-Zeager}
	\xmtitle{TITLE}
\mfpicnumber{1} \opengraphsfile{ExercisesforLinSystems} % mfpic settings added 


\label{ExercisesforLinSystems}

In Exercises \ref{triangfirst} - \ref{trianglast}, put each system of linear equations into triangular form and solve the system if possible.  Classify each system as consistent independent, consistent dependent, or inconsistent.

\begin{multicols}{2}
\begin{enumerate}


\item $\left\{ \begin{array}{rcr} -5x + y & = & 17  \\ x + y & = & 5  \end{array} \right.$ \label{triangfirst}
\item $\left\{ \begin{array}{rcr} x + y + z & = & 3 \\ 2x - y + z & = & 0 \\ -3x + 5y + 7z & = & 7  \end{array} \right.$

\setcounter{HW}{\value{enumi}}
\end{enumerate}
\end{multicols}



\begin{multicols}{2}
\begin{enumerate}
\setcounter{enumi}{\value{HW}}


\item \label{dependentsystemmuliple} $\left\{ \begin{array}{rcr} 4x - y + z & = & 5 \\ 2y + 6z & = & 30 \\ x + z & = & 5  \end{array} \right.$
\item $\left\{ \begin{array}{rcr} 4x - y + z & = & 5 \\ 2y + 6z & = & 30 \\ x + z & = & 6  \end{array} \right.$

\setcounter{HW}{\value{enumi}}
\end{enumerate}
\end{multicols}



\begin{multicols}{2}
\begin{enumerate}
\setcounter{enumi}{\value{HW}}

\item $\left\{ \begin{array}{rcr} x + y + z & = & -17  \\ y - 3z & = & 0  \end{array} \right.$


\item $\left\{ \begin{array}{rcr} x-2y+3z & = & 7 \\ -3x+y+2z & = & -5 \\ 2x+2y+z & = & 3  \end{array} \right.$


\setcounter{HW}{\value{enumi}}
\end{enumerate}
\end{multicols}



\begin{multicols}{2}
\begin{enumerate}
\setcounter{enumi}{\value{HW}}


\item $\left\{ \begin{array}{rcr} 3x-2y+z & = & -5 \\ x+3y-z & = & 12 \\ x+y+2z & = & 0  \end{array} \right.$
\item $\left\{ \begin{array}{rcr} 2x-y+z& = & -1 \\ 4x+3y+5z & = & 1 \\  5y+3z & = & 4 \end{array} \right.$


\setcounter{HW}{\value{enumi}}
\end{enumerate}
\end{multicols}



\begin{multicols}{2}
\begin{enumerate}
\setcounter{enumi}{\value{HW}}


\item $\left\{ \begin{array}{rcr} x-y+z & = & -4 \\ -3x+2y+4z & = & -5 \\ x-5y+2z & = & -18  \end{array} \right.$
\item $\left\{ \begin{array}{rcr} 2x-4y+z & = & -7 \\ x-2y+2z & = & -2 \\ -x+4y-2z & = & 3  \end{array} \right.$


\setcounter{HW}{\value{enumi}}
\end{enumerate}
\end{multicols}



\begin{multicols}{2}
\begin{enumerate}
\setcounter{enumi}{\value{HW}}


\item $\left\{ \begin{array}{rcr} 2x-y+z & = & 1 \\ 2x+2y-z & = & 1 \\ 3x+6y+4z & = & 9  \end{array} \right.$
\item $\left\{ \begin{array}{rcr} x-3y-4z & = & 3 \\ 3x+4y-z & = & 13 \\ 2x-19y-19z & = & 2  \end{array} \right.$


\setcounter{HW}{\value{enumi}}
\end{enumerate}
\end{multicols}



\begin{multicols}{2}
\begin{enumerate}
\setcounter{enumi}{\value{HW}}


\item $\left\{ \begin{array}{rcr} x+y+z & = & 4 \\ 2x-4y-z& = & -1 \\ x-y & = & 2 \end{array} \right.$
\item $\left\{ \begin{array}{rcr} x-y+z & = & 8 \\ 3x+3y-9z & = & -6 \\  7x-2y+5z & = & 39 \end{array} \right.$


\setcounter{HW}{\value{enumi}}
\end{enumerate}
\end{multicols}



\begin{multicols}{2}
\begin{enumerate}
\setcounter{enumi}{\value{HW}}


\item $\left\{ \begin{array}{rcr} 2x-3y+z & = & -1 \\ 4x-4y+4z & = & -13 \\ 6x-5y+7z & = & -25  \end{array} \right.$

\item  $\left\{ \begin{array}{rcr} 2x_{\mbox{\tiny$1$}} + x_{\mbox{\tiny$2$}} - 12x_{\mbox{\tiny$3$}} -  x_{\mbox{\tiny$4$}} & = & 16 \\ 
-x_{\mbox{\tiny$1$}} + x_{\mbox{\tiny$2$}} + 12x_{\mbox{\tiny$3$}} - 4x_{\mbox{\tiny$4$}} & = & -5  \\  
3x_{\mbox{\tiny$1$}} +  2x_{\mbox{\tiny$2$}} - 16x_{\mbox{\tiny$3$}} - 3x_{\mbox{\tiny$4$}} & = & 25 \\
x_{\mbox{\tiny$1$}} +  2x_{\mbox{\tiny$2$}} - 5x_{\mbox{\tiny$4$}} & = & 11  \end{array} \right.$

\setcounter{HW}{\value{enumi}}
\end{enumerate}
\end{multicols}

\begin{multicols}{2}
\begin{enumerate}
\setcounter{enumi}{\value{HW}}



\item  $\left\{ \begin{array}{rcr} x_{\mbox{\tiny$1$}} - x_{\mbox{\tiny$3$}} & = & -2 \\ 
2x_{\mbox{\tiny$2$}} - x_{\mbox{\tiny$4$}} & = & 0  \\  
x_{\mbox{\tiny$1$}} -  2x_{\mbox{\tiny$2$}} + x_{\mbox{\tiny$3$}} & = & 0 \\
-x_{\mbox{\tiny$3$}} + x_{\mbox{\tiny$4$}} & = & 1  \end{array} \right.$

\item  $\left\{ \begin{array}{rcr} x_{\mbox{\tiny$1$}} - x_{\mbox{\tiny$2$}} - 5x_{\mbox{\tiny$3$}} +  3x_{\mbox{\tiny$4$}} & = & -1 \\ 
x_{\mbox{\tiny$1$}} + x_{\mbox{\tiny$2$}} + 5x_{\mbox{\tiny$3$}} - 3x_{\mbox{\tiny$4$}} & = & 0  \\  
x_{\mbox{\tiny$2$}} + 5x_{\mbox{\tiny$3$}} - 3x_{\mbox{\tiny$4$}} & = & 1 \\
x_{\mbox{\tiny$1$}} -  2x_{\mbox{\tiny$2$}} - 10x_{\mbox{\tiny$3$}} + 6x_{\mbox{\tiny$4$}} & = & -1  \end{array} \right.$ \label{trianglast}

\setcounter{HW}{\value{enumi}}
\end{enumerate}
\end{multicols}


\begin{enumerate}
\setcounter{enumi}{\value{HW}}

\item Find two other forms of the parametric solution to Exercise \ref{dependentsystemmuliple} above by reorganizing the equations so that $x$ or $y$ can be the free variable.

\item \label{herbalteablend} At The Crispy Critter's Head Shop and Patchouli Emporium along with their dried up weeds, sunflower seeds and astrological postcards they sell an herbal tea blend.  By weight, Type I herbal tea is 30\% peppermint, 40\% rose hips and 30\% chamomile, Type II has percents 40\%, 20\% and 40\%, respectively, and Type III has percents 35\%, 30\% and 35\%, respectively.  How much of each Type of tea is needed to make 2 pounds of a new blend of tea that is equal parts peppermint, rose hips and chamomile?  

\item Discuss with your classmates how you would approach Exercise \ref{herbalteablend} above if they needed to use up a pound of Type I tea to make room on the shelf for a new canister.

\item If you were to try to make 100 mL of a $60\%$ acid solution using stock solutions at $20\%$ and $40\%$, respectively, what would the triangular form of the resulting system look like?  Explain.

\end{enumerate}

\newpage

\subsection{Answers}


Because triangular form is not unique, we give only one possible answer to that part of the question.  Yours may be different and still be correct.

\begin{enumerate}

%%TODO \begin{multicols}{2} \raggedcolumns

\item $\left\{ \begin{array}{rcr} x + y & = & 5  \\ y & = & 7  \end{array} \right.$ 

Consistent independent\\
Solution $(-2, 7)$

% \end{multicols}

% \begin{multicols}{2} \raggedcolumns

\item $\left\{ \begin{array}{rcr} x - \frac{5}{3}y - \frac{7}{3}z & = & -\frac{7}{3} \\ [3pt] y + \frac{5}{4}z & = & 2 \\ z & = & 0  \end{array} \right.$

Consistent independent\\
Solution $(1, 2, 0)$

% \end{multicols}

% \begin{multicols}{2} \raggedcolumns

\item $\left\{ \begin{array}{rcr} x - \frac{1}{4}y + \frac{1}{4}z & = & \frac{5}{4} \\ [3pt] y + 3z & = & 15 \\ 0 & = & 0  \end{array} \right.$

Consistent dependent\\
Solution $(-t + 5, -3t + 15, t)$\\
for all real numbers $t$

% \end{multicols}

% \begin{multicols}{2} \raggedcolumns

\item $\left\{ \begin{array}{rcr} x - \frac{1}{4}y + \frac{1}{4}z & = & \frac{5}{4} \\ [3pt] y + 3z & = & 15 \\ 0 & = & 1 \end{array} \right.$

Inconsistent\\
No solution

% \end{multicols}

% \begin{multicols}{2} \raggedcolumns

\item $\left\{ \begin{array}{rcr} x + y + z & = & -17  \\ y - 3z & = & 0  \end{array} \right.$
\vspace{.25in}

Consistent dependent\\
Solution $(-4t - 17, 3t, t)$\\
for all real numbers $t$

% \end{multicols}

% \begin{multicols}{2} \raggedcolumns
\item $\left\{ \begin{array}{rcr} x-2y+3z & = & 7  \\ y - \frac{11}{5}z & = & -\frac{16}{5} \\ z & = & 1 \\  \end{array} \right.$
\vspace{.25in}

Consistent independent\\
Solution $(2,-1,1)$

% \end{multicols}

% \begin{multicols}{2} \raggedcolumns
\item $\left\{ \begin{array}{rcr} x+y+2z & = & 0  \\ y - \frac{3}{2}z & = & 6 \\ z & = & -2 \\  \end{array} \right.$
\vspace{.25in}

Consistent independent\\
Solution $(1,3,-2)$

% \end{multicols}


% \begin{multicols}{2} \raggedcolumns
\item $\left\{ \begin{array}{rcr} x - \frac{1}{2} y + \frac{1}{2} z & = & -\frac{1}{2}  \\ [3pt] y + \frac{3}{5} z & = & \frac{3}{5} \\ 0 & = & 1 \\  \end{array} \right.$
\vspace{.25in}

Inconsistent\\
no solution


% \end{multicols}


% \begin{multicols}{2} \raggedcolumns
\item $\left\{ \begin{array}{rcr} x-y+z & = & -4  \\ y - 7z & = & 17 \\ z & = & -2 \\  \end{array} \right.$
\vspace{.25in}

Consistent independent\\
Solution $(1,3,-2)$

% \end{multicols}

% \begin{multicols}{2} \raggedcolumns
\item $\left\{ \begin{array}{rcr} x-2y+2z & = & -2  \\ y  & = & \frac{1}{2} \\ z & = & 1 \\  \end{array} \right.$
\vspace{.25in}

Consistent independent\\
Solution $\left(-3,\frac{1}{2},1\right)$

% \end{multicols}

% \begin{multicols}{2} \raggedcolumns
\item $\left\{ \begin{array}{rcr} x-\frac{1}{2} y+\frac{1}{2} z & = & \frac{1}{2}  \\ [3pt] y - \frac{2}{3} z & = & 0 \\ z & = & 1 \\  \end{array} \right.$
\vspace{.25in}

Consistent independent\\
Solution $\left(\frac{1}{3},\frac{2}{3},1\right)$

% \end{multicols}


% \begin{multicols}{2} \raggedcolumns
\item $\left\{ \begin{array}{rcr} x-3y-4z & = & 3  \\ y + \frac{11}{13} z & = & \frac{4}{13} \\ 0 & = & 0 \\  \end{array} \right.$
\vspace{.25in}

Consistent dependent\\
Solution $\left(\frac{19}{13} t + \frac{51}{13},-\frac{11}{13} t+\frac{4}{13},t\right)$\\
for all real numbers $t$

% \end{multicols}

% \begin{multicols}{2} \raggedcolumns
\item $\left\{ \begin{array}{rcr} x+y+z & = & 4  \\ y + \frac{1}{2} z & = & \frac{3}{2} \\ 0 & = & 1 \\  \end{array} \right.$
\vspace{.25in}

Inconsistent\\
no solution


% \end{multicols}

% \begin{multicols}{2} \raggedcolumns
\item $\left\{ \begin{array}{rcr} x-  y +  z & = & 8  \\ y -2z & = & -5 \\ z & = & 1 \\  \end{array} \right.$
\vspace{.25in}

Consistent independent\\
Solution $\left(4,-3,1\right)$


% \end{multicols}


% \begin{multicols}{2} \raggedcolumns
\item $\left\{ \begin{array}{rcr} x- \frac{3}{2} y + \frac{1}{2} z & = & -\frac{1}{2}  \\[3pt] y +  z & = & -\frac{11}{2} \\ 0 & = & 0 \\  \end{array} \right.$
\vspace{.25in}

Consistent dependent\\
Solution $\left(-2t - \frac{35}{4},-t - \frac{11}{2},t\right)$\\
for all real numbers $t$

% \end{multicols}


% \begin{multicols}{2} \raggedcolumns

\item  $\left\{ \begin{array}{rcr} x_{\mbox{\tiny$1$}} + \frac{2}{3}x_{\mbox{\tiny$2$}} - \frac{16}{3}x_{\mbox{\tiny$3$}} -  x_{\mbox{\tiny$4$}} & = & \frac{25}{3} \\ [3pt]
x_{\mbox{\tiny$2$}} + 4x_{\mbox{\tiny$3$}} - 3x_{\mbox{\tiny$4$}} & = & 2  \\  
0 & = & 0 \\
0 & = & 0  \end{array} \right.$

Consistent dependent\\
Solution $(8s - t + 7, -4s + 3t + 2, s, t)$\\
for all real numbers $s$ and $t$

% \end{multicols}

% \begin{multicols}{2} \raggedcolumns

\item  $\left\{ \begin{array}{rcr} x_{\mbox{\tiny$1$}} - x_{\mbox{\tiny$3$}} & = & -2 \\ [3pt]
x_{\mbox{\tiny$2$}} - \frac{1}{2}x_{\mbox{\tiny$4$}} & = & 0  \\ [3pt]
x_{\mbox{\tiny$3$}} - \frac{1}{2} x_{\mbox{\tiny$4$}} & = & 1 \\ [3pt]
x_{\mbox{\tiny$4$}} & = & 4  \end{array} \right.$

Consistent independent\\
Solution $(1, 2, 3, 4)$

% \end{multicols}

% \begin{multicols}{2} \raggedcolumns

\item  $\left\{ \begin{array}{rcr} x_{\mbox{\tiny$1$}} - x_{\mbox{\tiny$2$}} - 5x_{\mbox{\tiny$3$}} +  3x_{\mbox{\tiny$4$}} & = & -1 \\ 
x_{\mbox{\tiny$2$}} + 5x_{\mbox{\tiny$3$}} - 3x_{\mbox{\tiny$4$}} & = & \frac{1}{2}  \\  
0 & = & 1 \\
0 & = & 0 \end{array} \right.$

Inconsistent\\
No solution

% \end{multicols}

\item If $x$ is the free variable then the solution is $(t, 3t, -t + 5)$ and if $y$ is the free variable then the solution is $\left(\frac{1}{3}t, t, -\frac{1}{3}t + 5\right)$.


\item $\frac{4}{3}- \frac{1}{2}t$ pounds of Type I, $\frac{2}{3} - \frac{1}{2}t$ pounds of Type II and $t$ pounds of Type III where $0 \leq t \leq \frac{4}{3}$.

\end{enumerate}

\end{document}
