\documentclass{ximera}

\begin{document}
	\author{Stitz-Zeager}
	\xmtitle{Exercises for App Factoring}{}

\mfpicnumber{1} \opengraphsfile{ExercisesforAppFactoring} % mfpic settings added 


\label{ExercisesforAppFactoring}

In Exercises \ref{factoringexfirst} - \ref{factoringexlast}, factor completely over the integers.  Check your answer by multiplication.

\begin{multicols}{3}
\begin{enumerate}

\item $2x - 10x^2$ \label{factoringexfirst}
\item $12t^5 - 8t^3$
\item $16xy^2 - 12x^2y$

\setcounter{HW}{\value{enumi}}
\end{enumerate}
\end{multicols}

\begin{multicols}{3}
\begin{enumerate}
\setcounter{enumi}{\value{HW}}

\item $5(m+3)^2- 4(m+3)^3$
\item $(2x-1)(x+3) - 4(2x-1)$
\item $t^2(t-5) + t - 5$

\setcounter{HW}{\value{enumi}}
\end{enumerate}
\end{multicols}

\begin{multicols}{3}
\begin{enumerate}
\setcounter{enumi}{\value{HW}}

\item $w^2 - 121$
\item $49 - 4t^2$
\item $81t^4 - 16$

\setcounter{HW}{\value{enumi}}
\end{enumerate}
\end{multicols}

\begin{multicols}{3}
\begin{enumerate}
\setcounter{enumi}{\value{HW}}

\item $9z^2 - 64y^4$
\item $(y+3)^2 - 4y^2$
\item $(x+h)^3 - (x+h)$

\setcounter{HW}{\value{enumi}}
\end{enumerate}
\end{multicols}

\begin{multicols}{3}
\begin{enumerate}
\setcounter{enumi}{\value{HW}}

\item $y^2 - 24y + 144$
\item $25t^2 + 10t + 1$
\item $12x^3 - 36x^2 + 27x$

\setcounter{HW}{\value{enumi}}
\end{enumerate}
\end{multicols}

\begin{multicols}{3}
\begin{enumerate}
\setcounter{enumi}{\value{HW}}

\item $m^4 + 10m^2 + 25$
\item $27 - 8x^3$
\item $t^6 +t^3$


\setcounter{HW}{\value{enumi}}
\end{enumerate}
\end{multicols}



\begin{multicols}{3}
\begin{enumerate}
\setcounter{enumi}{\value{HW}}

\item $x^2 - 5x - 14$
\item $y^2 - 12y + 27$
\item $3t^2 + 16t + 5$


\setcounter{HW}{\value{enumi}}
\end{enumerate}
\end{multicols}


\begin{multicols}{3}
\begin{enumerate}
\setcounter{enumi}{\value{HW}}

\item $6x^2 - 23x + 20$
\item $35+2m - m^2$
\item $7w - 2w^2 - 3$



\setcounter{HW}{\value{enumi}}
\end{enumerate}
\end{multicols}


\begin{multicols}{3}
\begin{enumerate}
\setcounter{enumi}{\value{HW}}

\item $3m^3 + 9m^2 - 12m$
\item $x^4 + x^2 - 20$
\item $4(t^2-1)^2 +3(t^2-1) - 10$


\setcounter{HW}{\value{enumi}}
\end{enumerate}
\end{multicols}

\begin{multicols}{3}
\begin{enumerate}
\setcounter{enumi}{\value{HW}}

\item $x^3 - 5x^2 - 9x + 45$
\item $3t^2 + t - 3 - t^3$
\item\hspace{-0.1in}\footnote{$y^4 + 5y^2 + 9 = (y^4 + 6y^2 + 9) - y^2$} $y^4 + 5y^2 + 9$\label{factoringexlast}


\setcounter{HW}{\value{enumi}}
\end{enumerate}
\end{multicols}

In Exercises \ref{solvebyfactorfirst} - \ref{solvebyfactorlast},  find all rational number solutions.  Check your answers.

\begin{multicols}{3}
\begin{enumerate}
\setcounter{enumi}{\value{HW}}

\item   $(7x+3)(x-5) = 0$ \label{solvebyfactorfirst}
\item   $(2t-1)^2 (t+4) = 0$
\item   $(y^2 + 4)(3y^2 +y - 10) = 0$

\setcounter{HW}{\value{enumi}}
\end{enumerate}
\end{multicols}


\begin{multicols}{3}
\begin{enumerate}
\setcounter{enumi}{\value{HW}}

\item   $4t = t^2$
\item   $y+3 = 2y^2$
\item   $26x = 8x^2 + 21$  

\setcounter{HW}{\value{enumi}}
\end{enumerate}
\end{multicols}


\begin{multicols}{3}
\begin{enumerate}
\setcounter{enumi}{\value{HW}}

\item $16x^4 = 9x^2$
\item $w(6w+11) = 10$
\item $2w^2 + 5w + 2 = - 3(2w+1)$

\setcounter{HW}{\value{enumi}}
\end{enumerate}
\end{multicols}


\begin{multicols}{3}
\begin{enumerate}
\setcounter{enumi}{\value{HW}}

\item $x^2(x-3) = 16(x-3)$
\item $(2t+1)^3 = (2t+1)$
\item $a^4 + 4 = 6 - a^2$

\setcounter{HW}{\value{enumi}}
\end{enumerate}
\end{multicols}

\begin{multicols}{3}
\begin{enumerate}
\setcounter{enumi}{\value{HW}}

\item $\dfrac{8t^2}{3} = 2t+3$\vphantom{$\dfrac{y^4}{3} - y^2 = \dfrac{3}{2} (y^2 + 3)$}
\item $\dfrac{x^3+x}{2} = \dfrac{x^2+1}{3}$\vphantom{$\dfrac{y^4}{3} - y^2 = \dfrac{3}{2} (y^2 + 3)$}
\item $\dfrac{y^4}{3} - y^2 = \dfrac{3}{2} (y^2 + 3)$ \label{solvebyfactorlast}

\setcounter{HW}{\value{enumi}}
\end{enumerate}
\end{multicols}

\begin{enumerate}
\setcounter{enumi}{\value{HW}}

\item  With help from your classmates, factor $4x^4 + 8x^2 + 9$.  

\item  With help from your classmates, find an equation which has $3$, $-\frac{1}{2}$, and $117$ as solutions.  

\setcounter{HW}{\value{enumi}}
\end{enumerate}

\newpage

\subsection{Answers}

\begin{multicols}{3}
\begin{enumerate}

\item $2x(1 - 5x)$ 
\item $4t^3(3t^2-2)$
\item $4xy(4y-3x)$

\setcounter{HW}{\value{enumi}}
\end{enumerate}
\end{multicols}

\begin{multicols}{3}
\begin{enumerate}
\setcounter{enumi}{\value{HW}}

\item $-(m+3)^2(4m+7)$
\item $(2x-1)(x-1)$
\item $(t-5)(t^2+1)$

\setcounter{HW}{\value{enumi}}
\end{enumerate}
\end{multicols}

\begin{multicols}{3}
\begin{enumerate}
\setcounter{enumi}{\value{HW}}

\item $(w-11)(w+11)$
\item $(7-2t)(7+2t)$
\item $(3t-2)(3t+2)(9t^2+4)$

\setcounter{HW}{\value{enumi}}
\end{enumerate}
\end{multicols}

\begin{multicols}{3}
\begin{enumerate}
\setcounter{enumi}{\value{HW}}

\item $(3z-8y^2)(3z+8y^2)$
\item $-3(y - 3)(y+1)$
\item $(x+h)(x+h-1)(x+h+1)$

\setcounter{HW}{\value{enumi}}
\end{enumerate}
\end{multicols}

\begin{multicols}{3}
\begin{enumerate}
\setcounter{enumi}{\value{HW}}

\item $(y-12)^2$
\item $(5t+1)^2$
\item $3x(2x-3)^2$

\setcounter{HW}{\value{enumi}}
\end{enumerate}
\end{multicols}

\begin{multicols}{3}
\begin{enumerate}
\setcounter{enumi}{\value{HW}}

\item $(m^2+5)^2$
\item $(3-2x)(9 + 6x + 4x^2)$
\item $t^3(t+1)(t^2 - t + 1)$


\setcounter{HW}{\value{enumi}}
\end{enumerate}
\end{multicols}



\begin{multicols}{3}
\begin{enumerate}
\setcounter{enumi}{\value{HW}}

\item $(x-7)(x+2)$
\item $(y-9)(y-3)$
\item $(3t+1)(t+5)$


\setcounter{HW}{\value{enumi}}
\end{enumerate}
\end{multicols}


\begin{multicols}{3}
\begin{enumerate}
\setcounter{enumi}{\value{HW}}

\item $(2x-5)(3x-4)$
\item $(7-m)(5+m)$
\item $(-2w+1)(w-3)$



\setcounter{HW}{\value{enumi}}
\end{enumerate}
\end{multicols}


\begin{multicols}{3}
\begin{enumerate}
\setcounter{enumi}{\value{HW}}

\item $3m(m-1)(m+4)$
\item $(x-2)(x+2)(x^2+5)$
\item $(2t-3)(2t+3)(t^2+1)$


\setcounter{HW}{\value{enumi}}
\end{enumerate}
\end{multicols}

\begin{multicols}{3}
\begin{enumerate}
\setcounter{enumi}{\value{HW}}

\item $(x-3)(x+3)(x-5)$
\item $(t-3)(1-t)(1+t)$
\item $(y^2-y+3)(y^2+y+3)$


\setcounter{HW}{\value{enumi}}
\end{enumerate}
\end{multicols}



\begin{multicols}{3}
\begin{enumerate}
\setcounter{enumi}{\value{HW}}

\item   $x = -\dfrac{3}{7}$ or $x = 5$ 
\item   $t = \dfrac{1}{2}$ or $t = -4$
\item   $y = \dfrac{5}{3}$ or $y = -2$

\setcounter{HW}{\value{enumi}}
\end{enumerate}
\end{multicols}


\begin{multicols}{3}
\begin{enumerate}
\setcounter{enumi}{\value{HW}}

\item   $t = 0$ or $t = 4$\vphantom{$x = \dfrac{3}{2}$ or $x = \dfrac{7}{4}$ }
\item   $y = -1$ or $y = \dfrac{3}{2}$ \vphantom{$x = \dfrac{3}{2}$ or $x = \dfrac{7}{4}$}
\item   $x = \dfrac{3}{2}$ or $x = \dfrac{7}{4}$ 

\setcounter{HW}{\value{enumi}}
\end{enumerate}
\end{multicols}


\begin{multicols}{3}
\begin{enumerate}
\setcounter{enumi}{\value{HW}}

\item $x = 0$ or $x = \pm \dfrac{3}{4}$ 
\item $w = -\dfrac{5}{2}$ or $w = \dfrac{2}{3}$
\item $w=-5$ or $w = -\dfrac{1}{2}$

\setcounter{HW}{\value{enumi}}
\end{enumerate}
\end{multicols}


\begin{multicols}{3}
\begin{enumerate}
\setcounter{enumi}{\value{HW}}

\item $x=3$ or $x = \pm 4$ \vphantom{$t = -1$, $t= -\dfrac{1}{2}$, or $t = 0$}
\item $t = -1$, $t= -\dfrac{1}{2}$, or $t = 0$
\item $a = \pm 1$\vphantom{$t = -1$, $t= -\dfrac{1}{2}$, or $t = 0$}

\setcounter{HW}{\value{enumi}}
\end{enumerate}
\end{multicols}

\begin{multicols}{3}
\begin{enumerate}
\setcounter{enumi}{\value{HW}}

\item $t = -\dfrac{3}{4}$ or $t = \dfrac{3}{2}$
\item $x = \dfrac{2}{3}$
\item $y = \pm 3$  \vphantom{$x = \dfrac{2}{3}$}
\setcounter{HW}{\value{enumi}}
\end{enumerate}
\end{multicols}

\end{document}
