\documentclass{ximera}

\begin{document}
	\author{Stitz-Zeager}
	\xmtitle{Answers}
\mfpicnumber{1} \opengraphsfile{ExercisesforComplexZeros} % mfpic settings added 


\subsection{Answers}


\begin{enumerate}


\item $f(x) = x^2-4x+13 = (x-(2+3i)) (x-(2-3i))$ \\
Zeros: $x = 2 \pm 3i$ 
\item $f(x) = x^2 - 2x + 5 = (x-(1+2i))(x-(1-2i))$ \\ 
Zeros:  $x = 1 \pm 2i$


\item $p(z) = 3z^2 + 2z +10 = 3\left(z-\left(-\frac{1}{3} + \frac{\sqrt{29}}{3} i\right) \right) \left(z-\left(-\frac{1}{3} - \frac{\sqrt{29}}{3} i\right) \right)$
Zeros:  $z = -\frac{1}{3} \pm \frac{\sqrt{29}}{3} i$
\item $p(z) = z^3-2z^2+9z-18 = (z-2) \left(z^2+9\right) = (z-2)(z-3i)(z+3i)$\\
Zeros:  $z=2, \pm 3i$

\item $g(t) = t^{3} + 6t^{2} + 6t + 5 = (t + 5)(t^{2} + t + 1) = (t + 5) \left( t - \left( -\frac{1}{2} + \frac{\sqrt{3}}{2}i \right) \right) \left( t - \left(-\frac{1}{2} - \frac{\sqrt{3}}{2}i \right) \right)$ \\
Zeros: $t = -5, \;  t = -\frac{1}{2} \pm \frac{\sqrt{3}}{2}i $
\item $g(t) = 3t^{3} - 13t^{2} + 43t - 13 = (3t - 1)(t^{2} - 4t + 13) = (3t - 1)(t - (2 + 3i))(t - (2 - 3i))$\\
Zeros: $t = \frac{1}{3}, \; t = 2 \pm 3i$



\item $f(x) = x^3 + 3x^2 + 4x + 12 = (x+3) \left(x^2 + 4 \right) = (x+3)(x+2i)(x-2i)$ \\
Zeros:  $x = -3, \; \pm 2i$
\item $f(x) = 4x^3-6x^2-8x+15 = \left(x + \frac{3}{2} \right) \left(4x^2-12x+10\right) \\
 \phantom{f(x)} = 4 \left(x + \frac{3}{2} \right) \left(x - \left( \frac{3}{2} + \frac{1}{2}i  \right) \right) \left(x - \left( \frac{3}{2} - \frac{1}{2}i  \right) \right)$\\
Zeros:  $x = - \frac{3}{2}, \; x = \frac{3}{2} \pm \frac{1}{2}i$


\item  $p(z) = z^3 + 7z^2+9z-2 = (z+2) \left(z - \left( -\frac{5}{2}+\frac{\sqrt{29}}{2}\right) \right) \left(z - \left( -\frac{5}{2}-\frac{\sqrt{29}}{2}\right) \right)$ \\
Zeros:  $z = -2, \; z = -\frac{5}{2} \pm \frac{\sqrt{29}}{2}$
\item  $p(z) = 9z^3+2z+1 = \left(z + \frac{1}{3}\right) \left(9z^2 - 3z + 3\right) \\
\phantom{f(z)}= 9\left(z + \frac{1}{3}\right) \left(z - \left(\frac{1}{6} + \frac{\sqrt{11}}{6} i \right) \right) \left(z - \left(\frac{1}{6} - \frac{\sqrt{11}}{6} i \right) \right)$\\
Zeros:  $z = -\frac{1}{3}, \; z = \frac{1}{6} \pm \frac{\sqrt{11}}{6} i$

\item $g(t) = 4t^{4} - 4t^{3} + 13t^{2} - 12t + 3 = \left(t - \frac{1}{2}\right)^{2}\left(4t^{2} + 12\right) = 4\left(t - \frac{1}{2}\right)^{2}(t + i\sqrt{3})(t - i\sqrt{3})$\\
Zeros: $t = \frac{1}{2}, \; t = \pm \sqrt{3}i$
\item $g(t) = 2t^4-7t^3+14t^2-15t+6 = (t-1)^2 \left(2t^2 - 3t + 6\right)  \\
\phantom{f(t)} = 2 (t-1)^2 \left( t - \left( \frac{3}{4} +  \frac{\sqrt{39}}{4} i \right) \right)  \left( t - \left( \frac{3}{4} -  \frac{\sqrt{39}}{4} i \right) \right) $ \\
Zeros: $t = 1, \; t = \frac{3}{4}  \pm  \frac{\sqrt{39}}{4} i$



\item  $f(x) = x^4+x^3+7x^2+9x-18 = (x+2)(x-1)\left(x^2+9\right) = (x+2)(x-1)(x+3i)(x-3i)$\\
Zeros:  $x = -2, \; 1, \; \pm 3i$
\item  $f(x) = 6x^4+17x^3-55x^2+16x+12 = 6 \left(x + \frac{1}{3} \right) \left(x - \frac{3}{2} \right) \left(x - \left( -2 + 2 \sqrt{2}\right)\right) \left(x - \left( -2 - 2 \sqrt{2}\right)\right)$ \\
Zeros:  $x = -\frac{1}{3}, \; x = \frac{3}{2}, \; x = -2 \pm 2 \sqrt{2}$


\item  $p(z) = -3z^4-8z^3-12z^2-12z-5 = (z+1)^2 \left(-3z^2-2z-5\right) \\
\phantom{f(z)}= -3(z+1)^2\left(z - \left( -\frac{1}{3}+\frac{\sqrt{14}}{3} i\right) \right) \left(z - \left( -\frac{1}{3}-\frac{\sqrt{14}}{3} i\right) \right)$ \\
Zeros:  $z = -1, \; z = -\frac{1}{3} \pm \frac{\sqrt{14}}{3} i$
\item  $p(z) = 8z^4+50z^3+43z^2+2z-4 = 8\left(z + \frac{1}{2}\right) \left(z - \frac{1}{4}\right)(z - (-3 + \sqrt{5}))(z - (-3 - \sqrt{5}))$ \\
Zeros:  $z = -\frac{1}{2}, \; \frac{1}{4}, \; z = -3 \pm \sqrt{5}$

\item  $g(t) = t^4+9t^2+20 = \left(t^2+4\right) \left(t^2+5\right) = (t-2i)(t+2i)\left(t - i \sqrt{5}\right)\left(t + i \sqrt{5}\right)$\\
Zeros:  $t = \pm 2i, \pm i \sqrt{5}$
\item  $g(t) = t^4+5t^2-24 = \left(t^2-3 \right) \left(t^2+8\right) = (t-\sqrt{3})(t+\sqrt{3})\left(t - 2i \sqrt{2}\right)\left(t + 2i \sqrt{2}\right)$\\
Zeros:  $t = \pm \sqrt{3}, \pm 2i \sqrt{2}$

\item  $f(x) = x^5 - x^4+7x^3-7x^2+12x-12 = (x-1) \left(x^2 + 3\right) \left(x^2 + 4 \right) \\
\phantom{f(x)} = (x-1)(x - i \sqrt{3})(x + i \sqrt{3})(x-2i)(x+2i)$ \\
Zeros:  $x = 1, \;  \pm  \sqrt{3}i,  \; \pm 2i$
\item $f(x) = x^6 - 64 = (x-2)(x+2)\left(x^2+2x+4\right)\left(x^2-2x+4\right) \\
      \phantom{f(x)} = (x-2)(x+2)\left( x - \left( -1+i\sqrt{3} \right) \right)\left( x - \left( -1-i\sqrt{3} \right) \right)\left( x - \left( 1+i\sqrt{3} \right) \right)\left( x - \left( 1-i\sqrt{3} \right) \right)$ \\
Zeros:  $x = \pm 2$, $x = -1 \pm i\sqrt{3}$, $x = 1 \pm i\sqrt{3}$


\item $f(x) = x^{4} - 2x^{3} + 27x^{2} - 2x + 26 = (x^{2} - 2x + 26)(x^{2} + 1) = (x - (1 + 5i))(x - (1 - 5i))(x + i)(x - i)$\\ 
Zeros: $x = 1 \pm 5i, \; x = \pm i$
\item  $p(z) = 2z^4+5z^3+13z^2+7z+5 = \left(z^2+2z+5\right) \left(2z^2+z+1\right)  \\ \phantom{f(z)} = 2 (z-(-1+2i))(z-(-1-2i))\left(z - \left(-\frac{1}{4} + i \frac{\sqrt{7}}{4}\right) \right)\left(z - \left(-\frac{1}{4} - i \frac{\sqrt{7}}{4}\right) \right) $\\
Zeros:  $z = -1 \pm 2i, -\frac{1}{4} \pm i \frac{\sqrt{7}}{4}$

\setcounter{HW}{\value{enumi}}
\end{enumerate}

\begin{enumerate}
\setcounter{enumi}{\value{HW}}

\item $f(x) = 117(x+2)(x-2)(x+1)(x-1)$

\item $p(z)= -5(z-1)(z-3)^2$

\item  $g(t) = 7(t+3)^2(t-3)(t-6)$

\item $f(x) = -(x + 2)^{2}(x - 3)(x + 3)(x - 4)$

\item $p(z) = a(z+6)^2(z-1)(z-117)$ where $a$ can be any real number as long as $a<0$


\item $g(t) = 42(t-1)(t+1)(t-i)(t+i)$

\item $f(x) = 117(x+1)^2(x-2i)(x+2i)$

\item  $p(z) = -3(z-2)^2(z+2)(z-7i)(z+7i)$

\item $g(t) = a(t-6)(t-i)(t+i)(t-(1-3i))(t-(1+3i))$ where $a$ is any real number,  $a < 0$

\item $f(x) = -2(x-2i)(x+2i)(x+2)$

\setcounter{HW}{\value{enumi}}
\end{enumerate}

\begin{multicols}{3}
\begin{enumerate}
\setcounter{enumi}{\value{HW}}

\item $f(x) = x(x+6)(x-6)$

\item $g(t) = t(t+2)^3$

\item $p(z) = -2(z+1)(z-2)^2$

\setcounter{HW}{\value{enumi}}
\end{enumerate}
\end{multicols}


\begin{multicols}{3}
\begin{enumerate}
\setcounter{enumi}{\value{HW}}


\item $f(x) = 4\left(x+ \frac{1}{2}\right)^2 (x-3)$

\item $F(s)  =-s(s+2)^2$

\item $G(t) = t^3(t+2)^2$

\setcounter{HW}{\value{enumi}}
\end{enumerate}
\end{multicols}

\begin{multicols}{3}
\begin{enumerate}
\setcounter{enumi}{\value{HW}}


\item $f(x) =\frac{1}{2} (x-1)^2 (x+2)$
\item $p(t) =2 t^2 (t+2)^2$
\item $f(x) =-\frac{1}{2} (x-1) (x+2)^3$


\setcounter{HW}{\value{enumi}}
\end{enumerate}
\end{multicols}

\begin{enumerate}
\setcounter{enumi}{\value{HW}}

\item $p(t) = -\frac{1}{3} t(t+2)(t-3)$

\setcounter{HW}{\value{enumi}}
\end{enumerate}

\begin{enumerate}
\setcounter{enumi}{\value{HW}}

\item If $z = a+bi$, then $z$ corresponds to the point $(a,b)$ in the $xy$-plane.  Hence, $\overline{z} = \overline{a+bi} = a-bi$ corresponds to the point $(a,-b)$.  Hence, the points corresponding to $z$ and $\overline{z}$ are reflections about the $x$-axis.

\item    If $z = a+bi$, then $z$ corresponds to the point $(a,b)$ in the $xy$-plane.  Hence, $-z =-(a+bi) = -a-bi$ corresponds to the point $(-a,-b)$.  Hence, the points corresponding to $z$ and $-z$ are reflections through the origin.

\item  If $z = a+bi$, then $z$ corresponds to the point $(a,b)$ in the $xy$-plane.  Writing out the product $iz$, we get: $iz =i(a+bi) = ia+bi^2 = ia - b = -b+ia$.  Hence, $iz$ corresponds to the point $(-b,a)$.  If $z \neq 0$, then neither $a$ nor $b$ is $0$ (do you see why?) Hence, the slope of the line containing $(0,0)$ and $(a,b)$ is $\frac{b}{a}$ and the slope of the line containing $(0,0)$ and $(-b,a)$ is $-\frac{a}{b}$.  Per Theorem \ref{parallelperpendicularslopetheorem}, since the slopes of these lines are negative reciprocals, the lines themselves are perpendicular.\footnote{We'll be able to show in Section \ref{PolarComplex}  that, more precisely, multiplication by $i$ rotates the complex number counter-clockwise by $90^{\circ}$.}

\item $|z| = \sqrt{a^2+b^2}$ measures the distance from the origin to the point $(a,b)$.  Hence, $|z|$ measures the distance from $z$ to $0$ in the Complex Plane.  This is exactly how $|x|$ is defined in Definition \ref{absvaldistdefn} in Section \ref{AppAbsValEqIneq}.  In that section, however,  the only part of the Complex Plane under discussion is the real number line.

\setcounter{HW}{\value{enumi}}
\end{enumerate}




\end{document}
