\documentclass{ximera}

\begin{document}
	\author{Stitz-Zeager}
	\xmtitle{Exercises}
\mfpicnumber{1} \opengraphsfile{ExercisesforPolydivision} % mfpic settings added 



In Exercises \ref{synthdivreviewfirst} - \ref{synthdivreviewlast}, use synthetic division to perform the following polynomial divisions.  Identify the quotient and remainder. Write the divisor, quotient and remainder in the form given in Theorem \ref{polydivthm}.

\begin{multicols}{2}
\begin{enumerate}


\item $\left(3x^2-2x+1 \right) \div \left(x-1\right)$ \label{synthdivreviewfirst}
\item $\left(x^2-5 \right) \div \left(x-5\right)$

\setcounter{HW}{\value{enumi}}
\end{enumerate}
\end{multicols}

\begin{multicols}{2}
\begin{enumerate}
\setcounter{enumi}{\value{HW}}

\item $\left(3-4t-2t^2 \right) \div \left(t+1\right)$
\item $\left(4t^2-5t +3\right) \div \left(t+3\right)$

\setcounter{HW}{\value{enumi}}
\end{enumerate}
\end{multicols}

\begin{multicols}{2}
\begin{enumerate}
\setcounter{enumi}{\value{HW}}

\item $\left(z^3 + 8 \right) \div \left(z+2\right)$
\item $\left(4z^3 +2z-3 \right) \div \left(z -3\right)$

\setcounter{HW}{\value{enumi}}
\end{enumerate}
\end{multicols}

\begin{multicols}{2}
\begin{enumerate}
\setcounter{enumi}{\value{HW}}

\item $\left(18x^2-15x-25\right) \div \left(x - \frac{5}{3} \right)$
\item $\left(4x^2-1 \right) \div \left(x - \frac{1}{2} \right)$

\setcounter{HW}{\value{enumi}}
\end{enumerate}
\end{multicols}

\begin{multicols}{2}
\begin{enumerate}
\setcounter{enumi}{\value{HW}}

\item $\left(2t^3+t^2+2t+1 \right) \div \left(t + \frac{1}{2} \right)$
\item $\left(3t^3 - t + 4 \right) \div \left(t - \frac{2}{3} \right)$

\setcounter{HW}{\value{enumi}}
\end{enumerate}
\end{multicols}

\begin{multicols}{2}
\begin{enumerate}
\setcounter{enumi}{\value{HW}}

\item $\left(2z^3 - 3z +1 \right) \div \left(z - \frac{1}{2} \right)$
\item $\left(4z^4-12z^3+13z^2 -12z+9\right) \div \left(z - \frac{3}{2} \right)$

\setcounter{HW}{\value{enumi}}
\end{enumerate}
\end{multicols}

\begin{multicols}{2}
\begin{enumerate}
\setcounter{enumi}{\value{HW}}

\item $\left(x^4-6x^2+9 \right) \div \left(x -\sqrt{3} \right)$
\item $\left(x^6-6x^4+12x^2-8\right) \div \left(x +\sqrt{2} \right)$ \label{synthdivreviewlast}

\setcounter{HW}{\value{enumi}}
\end{enumerate}
\end{multicols}

In Exercises \ref{remainderexerfirst} - \ref{remainderexerlast}, find $p(c)$ using the Remainder Theorem.  If $p(c) = 0$, use the Factor Theorem to partially factor the polynomial function.

\begin{multicols}{2}
\begin{enumerate}
\setcounter{enumi}{\value{HW}}

\item $p(x) = 2x^2 - x + 1$, $c = 4$ \label{remainderexerfirst}
\item $p(x) = 4x^2-33x-180$, $c = 12$

\setcounter{HW}{\value{enumi}}
\end{enumerate}
\end{multicols}


\begin{multicols}{2}
\begin{enumerate}
\setcounter{enumi}{\value{HW}}

\item $p(t) = 2t^3 - t + 6$, $c=-3$
\item $p(t) = t^3+2t^2+3t+4$, $c =-1$

\setcounter{HW}{\value{enumi}}
\end{enumerate}
\end{multicols}

\begin{multicols}{2}
\begin{enumerate}
\setcounter{enumi}{\value{HW}}

\item $p(z) =3z^3-6z^2+4z-8$, $c=2$
\item $p(z) = 8z^3+12z^2+6z+1$, $c =-\frac{1}{2}$

\setcounter{HW}{\value{enumi}}
\end{enumerate}
\end{multicols}

\begin{multicols}{2}
\begin{enumerate}
\setcounter{enumi}{\value{HW}}

\item $p(x) = x^4 - 2x^2+4$, $c=\frac{3}{2}$
\item $p(x) = 6x^4-x^2+2$, $c =-\frac{2}{3}$

\setcounter{HW}{\value{enumi}}
\end{enumerate}
\end{multicols}


\begin{multicols}{2}
\begin{enumerate}
\setcounter{enumi}{\value{HW}}

\item $p(t) = t^4 +t^3-6t^2-7t-7$, $c=-\sqrt{7}$
\item $p(t) = t^2-4t+1$, $c =2-\sqrt{3}$ \label{remainderexerlast}

\setcounter{HW}{\value{enumi}}
\end{enumerate}
\end{multicols}



In Exercises \ref{factorpolyzerofirst} - \ref{factorpolyzerolast}, you are given a polynomial function and one of its zeros.  Find the remaining real zeros and factor the polynomial.  

\begin{multicols}{2}
\begin{enumerate}
\setcounter{enumi}{\value{HW}}

\item $x^{3} - 6x^{2} + 11x - 6, \;\; c = 1$ \label{factorpolyzerofirst}
\item $x^{3} - 24x^{2} + 192x - 512, \;\; c = 8$

\setcounter{HW}{\value{enumi}}
\end{enumerate}
\end{multicols}

\begin{multicols}{2}
\begin{enumerate}
\setcounter{enumi}{\value{HW}}

\item $3t^{3} + 4t^{2} - t - 2, \;\; c = \frac{2}{3}$
\item $2t^3-3t^2-11t+6, \;\; c=\frac{1}{2}$

\setcounter{HW}{\value{enumi}}
\end{enumerate}
\end{multicols}

\begin{multicols}{2}
\begin{enumerate}
\setcounter{enumi}{\value{HW}}

\item $z^3+2z^2-3z-6, \;\; c = -2$
\item $2z^3-z^2-10z+5, \;\; c=\frac{1}{2}$

\setcounter{HW}{\value{enumi}}
\end{enumerate}
\end{multicols}

\vspace*{-0.2in}
\enlargethispage{0.2in}
\begin{enumerate}
\setcounter{enumi}{\value{HW}}

\item $4x^{4} - 28x^{3} + 61x^{2} - 42x + 9$, $c = \frac{1}{2}$ is a zero of multiplicity 2 

\item  $t^5+2t^4-12t^3-38t^2-37t-12$, $c=-1$ is a zero of multiplicity 3

\item $125z^{5} - 275z^{4} - 2265z^{3} - 3213z^{2} - 1728z - 324$, $c = -\frac{3}{5}$ is a zero of multiplicity 3

\item $x^{2} - 2x - 2, \;\; c = 1 - \sqrt{3}$ \label{factorpolyzerolast}

\setcounter{HW}{\value{enumi}}
\end{enumerate}


\begin{enumerate}
\setcounter{enumi}{\value{HW}}

\item Find a quadratic polynomial with \underline{integer} coefficients which has $x = \dfrac{3}{5} \pm \dfrac{\sqrt{29}}{5}$ as its real zeros.

\item  \label{verifyrootsex}  For $f(x) = x^3 + 4x^2-5x-14$, show $f(-3-\sqrt{2}) = 0$ and $f(-3+\sqrt{2}) = 0$ two ways:

\begin{enumerate}

\item  By direct substitution.

\item  Using synthetic division and the Factor Theorem

\end{enumerate}

\item  \label{oneisazeroex} Let $f(x) = a_{n} x^{n} + a_{n-\mbox{\tiny$1$}} x^{n-\mbox{\tiny$1$}} + \ldots + a_{\mbox{\tiny $2$}} x^{\mbox{\tiny $2$}} + a_{\mbox{\tiny $1$}} x + a_{\mbox{\tiny $0$}}$ be a polynomial function with the property that $ a_{n}+a_{n-\mbox{\tiny$1$}} + \ldots + a_{\mbox{\tiny $1$}} + a_{\mbox{\tiny $0$}} = 0$.  (That is, the sum of the coefficients and the constant term is $0$.)  

Prove that $(x-1)$ is a factor of $f(x)$.

HINT:  Show $f(1) = 0$ and invoke the Factor Theorem

\item  Verify the result in number \ref{oneisazeroex} with the functions: $f(x) = x^3 - 2x + 1$ and  $f(x) = 3x^4-x-2$.

\item  \label{monomialdiffquotex} Suppose $a$ is a nonzero real number.  Find the quotients below, using synthetic division as required. 

\begin{multicols}{5}
\begin{itemize}

\item $\dfrac{x - a}{x-a}$ 

\item $\dfrac{x^2 - a^2}{x-a}$ 

\item $\dfrac{x^3 - a^3}{x-a}$ 

\item $\dfrac{x^4 - a^4}{x-a}$ 

\item $\dfrac{x^5 - a^5}{x-a}$ 


\end{itemize}

\end{multicols}

Based on the pattern that evolves, find the quotient: $\dfrac{x^{10} - a^{10}}{x-a}$.  What about  $\dfrac{x^{n} - a^{n}}{x-a}$?


\item  \label{geoseriespreview} Use your result from number \ref{monomialdiffquotex} to rewrite the sum: $1 + r + r^2 + \dots + r^{n-2} + r^{n-1}$ as a quotient. What assumptions need to be made about $r$?

\setcounter{HW}{\value{enumi}}
\end{enumerate}

\newpage

\subsection{Answers}


\begin{enumerate}

\item $\left(3x^2-2x+1 \right) = \left(x-1\right) (3x+1)+2$
\item $\left(x^2-5 \right)= \left(x-5\right)(x+5) + 20$


\item $\left(3-4t-2t^2 \right) = \left(t+1\right)(-2t-2)+5$
\item $\left(4t^2-5t +3\right) = \left(t+3\right)(4t-17)+54$


\item $\left(z^3 + 8 \right) = \left(z+2\right) \left(z^2-2z+4\right) + 0$
\item $\left(4z^3 +2z-3 \right) = \left(z -3\right) \left(4z^2+12z+38\right) + 111$


\item $\left(18x^2-15x-25\right) = \left(x - \frac{5}{3} \right)(18x+15)+0$
\item $\left(4x^2-1 \right) = \left(x - \frac{1}{2} \right)(4x+2)+0$


\item $\left(2t^3+t^2+2t+1 \right) = \left(t + \frac{1}{2} \right)\left(2t^2+2\right)+0$
\item $\left(3t^3 - t + 4 \right) = \left(t - \frac{2}{3} \right) \left(3t^2+2t+\frac{1}{3}\right) + \frac{38}{9}$


\item $\left(2z^3 - 3z +1 \right) = \left(z - \frac{1}{2} \right) \left(2z^2+z-\frac{5}{2}\right)-\frac{1}{4}$
\item $\left(4z^4-12z^3+13z^2 -12z+9\right) = \left(z - \frac{3}{2} \right) \left(4z^3-6z^2+4z-6 \right)+0$

\item $\left(x^4-6x^2+9 \right) = \left(x -\sqrt{3} \right) \left(x^3+\sqrt{3} \,x^2-3x-3\sqrt{3}\right) + 0$
\item $\left(x^6-6x^4+12x^2-8\right) = \left(x +\sqrt{2} \right) \left(x^5-\sqrt{2} \, x^4-4x^3+4\sqrt{2} \, x^2+4x-4\sqrt{2}\right) + 0$


\setcounter{HW}{\value{enumi}}
\end{enumerate}

\begin{multicols}{2}
\begin{enumerate}
\setcounter{enumi}{\value{HW}}

\item $p(4) = 29$
\item $p(12) =0$, $p(x) = (x-12)(4x+15)$

\setcounter{HW}{\value{enumi}}
\end{enumerate}
\end{multicols}


\begin{multicols}{2}
\begin{enumerate}
\setcounter{enumi}{\value{HW}}

\item $p(-3)=-45$
\item $p(-1)=2$

\setcounter{HW}{\value{enumi}}
\end{enumerate}
\end{multicols}

\begin{multicols}{2}
\begin{enumerate}
\setcounter{enumi}{\value{HW}}

\item $p(2) =0$, $p(z)= (z-2) \left(3z^2+4\right)$
\item $p\left(-\frac{1}{2}\right) = 0$, $p(z)  = \left(z+\frac{1}{2}\right)\left(8z^2+8z+2\right)$

\setcounter{HW}{\value{enumi}}
\end{enumerate}
\end{multicols}

\begin{multicols}{2}
\begin{enumerate}
\setcounter{enumi}{\value{HW}}

\item $p\left(\frac{3}{2}\right) = \frac{73}{16}$
\item $p\left(-\frac{2}{3}\right) = \frac{74}{27}$

\setcounter{HW}{\value{enumi}}
\end{enumerate}
\end{multicols}

\begin{enumerate}
\setcounter{enumi}{\value{HW}}

\item $p(-\sqrt{7}) = 0$, $p(t) = (t+\sqrt{7})\left(t^3+(1-\sqrt{7}) t^2+(1-\sqrt{7})t-\sqrt{7}  \right)$
\item $p(2-\sqrt{3}) =0$, $p(t) = (t-(2-\sqrt{3}))(t-(2+\sqrt{3})) $

\setcounter{HW}{\value{enumi}}
\end{enumerate}

\begin{enumerate}
\setcounter{enumi}{\value{HW}}

\item $x^{3} - 6x^{2} + 11x - 6 = (x - 1)(x - 2)(x - 3)$
\item $x^{3} - 24x^{2} + 192x - 512 = (x - 8)^{3}$
\item $3t^{3} + 4t^{2} - t - 2 = 3\left(t - \frac{2}{3}\right)(t + 1)^{2}$

\item $2t^3-3t^2-11t+6 = 2\left(t-\frac{1}{2}\right)(t+2)(t-3)$

\item $z^3+2z^2-3z-6 = (z+2)(z+\sqrt{3})(z-\sqrt{3})$
\item $2z^3-z^2-10z+5=2\left(z-\frac{1}{2}\right)(z+\sqrt{5})(z-\sqrt{5})$

\item $4x^{4} - 28x^{3} + 61x^{2} - 42x + 9 = 4\left(x - \frac{1}{2} \right)^{2}(x - 3)^{2}$

\item  $t^5+2t^4-12t^3-38t^2-37t-12 = (t+1)^3(t+3)(t-4)$

\item $125z^{5} - 275z^{4} - 2265z^{3} - 3213z^{2} - 1728z - 324$ = $125\left(z + \frac{3}{5} \right)^{3}(z + 2)(z - 6)$


\item $x^{2} - 2x - 2 = (x - (1 - \sqrt{3}))(x - (1 + \sqrt{3}))$

\item $p(x) = 5x^{2} - 6x - 4$

\addtocounter{enumi}{2}

\item  \begin{itemize}

\item For $f(x) = x^3 - 2x + 1$, the coefficients $1+(-2) + 1 = 0$ and $f(x) = (x-1)(x^2+x-1)$.

\item  For $f(x) = 3x^4-x-2$ the coefficients $3+(-1)+(-2) = 0$ and $f(x) = (x-1)(3x^3+3x^2+3x+2)$.

\end{itemize}

\item  \begin{multicols}{3}

\begin{itemize}

\item $\dfrac{x - a}{x-a} = 1$  \vphantom{$\dfrac{x^3 - a^3}{x-a} = x^2+ax+a^2$}

\item $\dfrac{x^2 - a^2}{x-a} = x+a$ \vphantom{$\dfrac{x^3 - a^3}{x-a} = x^2+ax+a^2$}

\item $\dfrac{x^3 - a^3}{x-a} = x^2+ax+a^2$ 

\end{itemize}

\end{multicols}

\begin{multicols}{2}

\begin{itemize}

\item $\dfrac{x^4 - a^4}{x-a} = x^3 + ax^2 + a^2x + a^3$ 

\item $\dfrac{x^5 - a^5}{x-a} = x^4+ax^3 + a^2x^2+a^3x+a^4$ 

\end{itemize}

\end{multicols}

Following the pattern: 

\begin{itemize}

\item $\dfrac{x^{10} - a^{10}}{x-a} = x^{9} + ax^8 + a^2x^7+a^3x^6+a^4x^5+a^5x^4+a^6x^3+a^7x^2+a^8x+a^9$

\item  $\dfrac{x^{n} - a^{n}}{x-a} = x^{n-1} + ax^{n-2} + a^2x^{n-3} + \ldots + a^{n-2} x + a^{n-1}$

\end{itemize}

\item Put $x=1$ and $a = r$ so that  $1 + r + r^2 + \dots + r^{n-2} + r^{n-1} = \dfrac{1 - r^{n}}{1-r}$.  Here,   $r \neq 1$ as otherwise we'd be dividing by $0$.

\setcounter{HW}{\value{enumi}}
\end{enumerate}



\end{document}
